dafny/prime.dfy
@@ -1,0 +1,107 @@
+include "modDiv.dfy"
+include "list.dfy"
+include "cycle.dfy"
+include "multiple.dfy"
+
+module Prime {
+
+    import ModDiv
+    import List
+
+    function method isPrimeLoop(prime: nat, loopValue: nat): bool 
+        requires loopValue > 0;
+        decreases loopValue;
+    {
+        if loopValue == 1 then true 
+        else if ModDiv.mod(prime, loopValue) == 0 then false
+        else isPrimeLoop(prime,loopValue - 1)
+    }
+
+    function method isPrime(prime: nat): bool
+    {
+        if prime < 2 then false
+        else isPrimeLoop(prime, prime - 1)
+    }
+
+    function method isPrimeSequence(list: seq<nat>): bool        
+    {
+        var allElementsArePrimes := forall k :: 0 <= k < |list| ==> isPrime(list[k]);
+        var allPrimesAreInTheList := |list| > 0 ==> 
+            forall v :: 2 <= v <= List.max(list) ==> ( 
+                isPrime(v) ==> exists k  :: 0 <= k < |list| && list[k] == v
+            );
+        var isSorted := List.sorted(list);
+        var isNonZero := List.nonZero(list);
+
+        if !isSorted then false
+        else if !isNonZero then false
+        else if !allElementsArePrimes then false
+        else if !allPrimesAreInTheList then false
+        else true
+    }
+
+    function method getPrimeSequenceUntil(value: nat): seq<nat>
+        ensures value < 2 ==> getPrimeSequenceUntil(value) == [];
+        ensures value >= 2 && !isPrime(value) ==> getPrimeSequenceUntil(value) == getPrimeSequenceUntil(value - 1);
+        ensures value >= 2 && isPrime(value) ==> |getPrimeSequenceUntil(value)| > 0;
+        ensures value >= 2 && isPrime(value) ==> getPrimeSequenceUntil(value)[0] == value;
+        decreases value;
+    {
+        var prev := if value < 2 then [] else getPrimeSequenceUntil(value - 1);
+        var primeSequence := if value < 2 then []
+        else if isPrime(value) then [value] + prev
+        else prev;
+
+        assert value < 2 ==> isPrime(value) == false;
+        assert isPrime(value) ==> primeSequence[0] == value;
+        assert value >= 2 && !isPrime(value) ==> primeSequence == getPrimeSequenceUntil(value - 1);
+        assert value >= 2 && isPrime(value)  ==> primeSequence[0] == value;
+
+        primeSequence
+    }
+
+    lemma getPrimeSequenceUntilValueIsPrimeSequence(value: nat, primeSequence: seq<nat>)
+        requires primeSequence == getPrimeSequenceUntil(value);
+        // ensures isPrimeSequence(primeSequence);
+    {
+        assert forall v :: 0 <= v < 2 ==> isPrime(v) == false;
+        if (value < 2) {
+            assert isPrimeSequence(primeSequence);
+        } else {
+            if (isPrime(value)) {
+                assert primeSequence[0] == value;
+                assert primeSequence[1..] == getPrimeSequenceUntil(value - 1);
+            } else {
+                assert primeSequence == getPrimeSequenceUntil(value - 1);
+            }
+            if (isPrime(value) && isPrime(value - 1))
+            {
+                assert primeSequence[0] == value;
+                assert primeSequence[1] == value - 1;
+                assert primeSequence[1] < primeSequence[0];
+            }
+            if (isPrime(value) && !isPrime(value - 1))
+            {
+                assert primeSequence[0] == value;
+                assert primeSequence[1..] == getPrimeSequenceUntil(value - 2);
+                getPrimeSequenceUntilValueIsPrimeSequence(value - 2, primeSequence[1..]);
+            }
+            if (!isPrime(value) && isPrime(value - 1))
+            {
+                assert primeSequence == getPrimeSequenceUntil(value - 1);
+                getPrimeSequenceUntilValueIsPrimeSequence(value - 1, primeSequence);
+            }
+            if (!isPrime(value) && !isPrime(value - 1))
+            {
+                assert primeSequence == getPrimeSequenceUntil(value - 2);
+                getPrimeSequenceUntilValueIsPrimeSequence(value - 2, primeSequence);
+            }
+            assert |primeSequence| > 1 ==> primeSequence[0] > primeSequence[1];
+        }
+    }
+
+    lemma thereIsSomePrimeBetweenAPrimeAndItSquared(prime: nat)
+    {
+
+    }
+}
